Dom.lean
@@ -36,6 +36,7 @@ import Dom.Properties.PreInsertValidity
 import Dom.Properties.Algorithms
 import Dom.Properties.Path
 import Dom.Properties.NodeQuery
+import Dom.Properties.RangeDelete
 import Dom.Properties.Range
 import Dom.Properties.Iterator
 import Dom.Properties.Walker
